Common.v
@@ -7,6 +7,7 @@ Require Import Sumbool.
 Require Import Basics.
 Require Import Omega.
 
+
 (* Some helpful lemmas regarding List *)
 
 (* If List.length l = 1, l = h::nil. *)
